

# MTH 320: HW 4

Lucky Chouhan

February 25, 2026

Problems from Abbott's book (2nd ed.) are labeled by **Abbott chpt.sec.#**.

1. **(Abbott 2.3.6)** Consider the sequence  $(b_n)$  given by  $b_n = n - \sqrt{n^2 + n}$ . Prove that  $(b_n)$  converges and find its limit. You may use the following facts freely: the Algebraic Limit Laws,  $\lim \frac{1}{n} = 0$ , and if  $\lim x_n = x$  then  $\lim \sqrt{x_n} = \sqrt{x}$ .

**Solution.** Rationalizing the sequence  $(b_n)$  gives,

$$b_n = \frac{-n}{n + \sqrt{n^2 + n}} = \frac{-1}{1 + \sqrt{1 + 1/n}}$$

Notice that for any  $n \in \mathbb{N}$ ,  $1 + 1/n \geq 1 + 1/(n+1) \implies b_n \geq b_{n+1}$ . Further,

$$\begin{aligned} 1 + \frac{1}{n} &\geq 1 \\ 1 + \sqrt{1 + \frac{1}{n}} &\geq 2 \\ b_n &\geq -\frac{1}{2}. \end{aligned}$$

Thus,  $(b_n)$  is decreasing and bounded. Therefore, by Monotone Convergence Theorem it converges.

Using algebraic properties of limits of sequences we see that,

$$\begin{aligned} \lim(b_n) &= \lim \left( \frac{-1}{1 + \sqrt{1 + 1/n}} \right) \\ &= \frac{\lim(-1)}{\lim(1 + \sqrt{1 + 1/n})} \\ \lim(b_n) &= -\frac{1}{1 + 1} = -\frac{1}{2}. \end{aligned}$$

2. **(Abbott 2.3.12)** In the following assume that  $(a_n)$  converges to  $a$  and determine the validity of each claim. If it is true then provide a proof and if it is false provide a counterexample.

- (a) Let  $X \subset \mathbb{R}$ . If  $a_n$  is an upper bound for  $X$  then  $a$  is an upper bound for  $X$ .
- (b) If  $a_n$  is in the complement of the set  $(0, 1)$  for all  $n$  then  $a$  is in the complement of  $(0, 1)$ .
- (c) If  $a_n$  is rational for all  $n$  then  $a$  is rational.

**Claim (a).** The claim is true.

**Proof.** For any  $x \in X$ , we have  $a_n \geq x$ . Define  $b_n = a_n - x \geq 0$ . From algebraic properties of limit  $\lim(b_n) = \lim(a_n - x) = \lim(a_n) - \lim(x) = a - x$ .

Take  $b = a - x$  and our goal is to prove that  $b \geq 0$ . Assume that  $b < 0$ . Since  $(b_n)$  converges to  $b$  then for  $\epsilon = |b|/2$  there exists an  $N \in \mathbb{N}$  so that  $|b_n - b| < |b|/2$  for all  $n \geq N$  that is  $b - |b|/2 < b_n < b + |b|/2 < 0$ .

But this contradicts the fact that  $b_n \geq 0$  for all  $n$ . Therefore,  $a - x = b \geq 0$  and  $a \geq x$ .

**Claim (b).** The claim is true.

**Proof.** Suppose for contradiction, the  $a \in (0, 1)$ , Let  $\epsilon = \min\{a, 1 - a\}/2 > 0$ . Then the  $\epsilon$ -neighborhood  $(a - \epsilon, a + \epsilon)$  is contained in  $(0, 1)$ . Since  $a_n \rightarrow a$ , there exists  $N$  such that for all  $n \geq N$ ,  $|a_n - a| < \epsilon$ , hence  $a_n \in (0, 1)$ . This contradicts the hypothesis that no  $a_n$  lies in  $(0, 1)$ . Therefore  $a \in (0, 1)$ .

**Claim (c).** The claim is false. **Counterexamples.** We can define sequence of rationals  $x_n = (1 + \frac{1}{n})^n$  for  $n \in \mathbb{N}$  and we also know that  $\lim x_n = e$  that is an irrational number.

Or we could have defined  $y_n = \lfloor 10^n \sqrt{2} \rfloor 10^{-n}$  for  $n \in \mathbb{N}$  and we can see that  $y_n \in \mathbb{Q}$  for each  $n$  but  $\lim y_n = \sqrt{2} \notin \mathbb{Q}$ .

### 3. (Abbott 2.4.1)

- (a) Let  $(x_n)$  be a sequence defined by  $x_1 = 3$  and

$$x_{n+1} = \frac{1}{4 - x_n}.$$

Prove that  $(x_n)$  converges.

- (b) From (a) we know  $\lim x_n$  exists. Why must  $x_{n+1}$  also exists and be equal to the same value?
- (c) Take the limit on both sides of the recursive equation in part (a) and explicitly compute  $\lim x_n$ .

**Proof. (a)** Assume that  $x_n \leq 1$  for all  $n \geq 2$ , evaluating  $x_2 = 1, x_3 = 1/3$  agree with our assumption,  $x_n \leq 1 \implies 4 - x_n \geq 3 \implies x_{n+1} \leq 1/3 \leq 1$ .

Now also assume that  $x_n \geq 0$  for all  $n$ . For  $n + 1$ ,  $4 - x_n \leq 4 \implies x_{n+1} \geq 1/4 \geq 0$ .

Therefore,  $x_n \in [1/4, 1]$  for all  $n \geq 2$ .

Consider the difference of two consecutive terms of sequence,

$$\begin{aligned} x_{n+1} - x_n &= \frac{1}{4 - x_n} - \frac{1}{4 - x_{n-1}} \\ &= \frac{x_n - x_{n-1}}{(4 - x_n)(4 - x_{n-1})} \end{aligned}$$

recursively applying the last relation gives us,

$$\begin{aligned} x_{n+1} - x_n &= \frac{-2}{(4 - x_n)(4 - x_{n-1})^2(4 - x_{n-2})^2 \cdots (4 - x_2)^2} \\ &= - \underbrace{\left( \frac{2 \cdot x_{n+1}}{(4 - x_{n-1})^2(4 - x_{n-2})^2 \cdots (4 - x_2)^2} \right)}_{\geq 0} \\ &\leq 0. \end{aligned}$$

Thus,  $(x_n)$  is a decreasing sequence bounded above by 1, therefore by Monotone Convergence Theorem it converges.

**Explanation (b).** Since we know  $(x_n)$  converges, say to  $x$ , that means, for any  $\epsilon > 0$ , we can find an  $N \in \mathbb{N}$  such that  $|x_n - x| < \epsilon$  for all  $n \geq N$ . Moreover,  $n + 1 \geq n \geq N$ , therefore,  $|x_{n+1} - x| < \epsilon$  for each  $\epsilon > 0$ . Hence,  $\lim(x_{n+1}) = \lim(x_n) = x$ .

**Computation (c).** Take  $\lim x_n = x$ . We've,

$$x_{n+1} = \frac{1}{4 - x_n}.$$

So,

$$x = \lim(x_{n+1}) = \lim \left( \frac{1}{4 - x_n} \right) = \frac{1}{4 - x}.$$

Solving, the equation  $x^2 - 4x + 1 = 0$  gives us  $x = 2 \pm \sqrt{3}$ . Since  $2 + \sqrt{3} = 3.732 \cdots \geq 3 \geq x_n$  for all  $n$ , therefore,  $x = 2 - \sqrt{3} = 0.2679 \dots$

4. (**Abbott 2.4.3**) Prove that the sequence  $(x_n)$  defined by  $x_1 = \sqrt{2}$  and  $x_{n+1} = \sqrt{2 + x_n}$  converges.

**Proof.** Notice that,  $x_1 = \sqrt{2} = 2 \cos(\pi/4)$  and using  $1 + \cos(\theta) = 2 \cos^2(\theta/2)$  for any  $\theta$ , we see that,

$$x_2 = \sqrt{2 + x_1} = \sqrt{2 + 2 \cos(\pi/4)} = \sqrt{4 \cos^2(\pi/8)} = 2 \cos(\pi/8).$$

Iterating this for all, we see that  $x_n = 2 \cos(\frac{\pi}{2^{n+1}})$  for any  $n$ . For  $n + 1$ ,

$$x_{n+1} = \sqrt{2 + x_n} = \sqrt{2 + 2 \cos \left( \frac{\pi}{2^{n+1}} \right)} = 2 \cos \left( \frac{\pi}{2^{n+2}} \right).$$

Further,  $\frac{\pi}{2^{n+1}} > \frac{\pi}{2^{n+2}}$  and we know that  $\cos(x)$  is a decreasing function in  $[0, \pi]$  therefore,  $\cos\left(\frac{\pi}{2^{n+1}}\right) \leq \cos\left(\frac{\pi}{2^{n+2}}\right)$  that is  $x_n \leq x_{n+1}$ .

Notice that,  $\cos(x) \leq 1$ , so is  $x_n$ . Thus, by Monotone Convergence Theorem  $x_n$  converges and its limit can be evaluated as,

$$\lim x_n = \lim \left( 2 \cos \left( \frac{\pi}{2^{n+1}} \right) \right) = 2.$$

5. **(Abbott 2.4.7)** Let  $(a_n)$  be a bounded sequence. Prove that the sequence defined by  $y_n = \sup\{a_k : k \geq n\}$  converges. (**Remark:** The limit superior of  $(a_n)$  is defined by  $\limsup a_n = \lim y_n$ .)

**Proof.** Since  $(a_n)$  is bounded, so there exists  $M \in \mathbb{N}$  such that  $a_n \geq M$  for all  $n \in \mathbb{N}$ . Moreover,  $y_n = \sup\{a_k : k \geq n\} \geq a_n \geq M$ , this tells us  $(y_n)$  is also bounded below by  $M$ .

We can also see  $y_n$  as,

$$\begin{aligned} y_n &= \sup\{a_k : k \geq n\} \\ &= \max\{a_n, \sup\{a_k : k \geq n+1\}\} \\ &= \max\{a_n, y_{n+1}\} \\ &\geq y_{n+1}. \end{aligned}$$

Thus,  $(y_n)$  is decreasing and bounded sequence, therefore by Monotone Convergence Theorem converges.

6. Establish the convergence of the sequence  $(y_n)$  defined by

$$y_n = \frac{1}{n+1} + \frac{1}{n+2} + \cdots + \frac{1}{n+n}.$$

**Proof.** Notice that,

$$y_n = \frac{1}{n+1} + \frac{1}{n+2} + \cdots + \frac{1}{n+n} \leq \frac{n}{n+1} \leq 1.$$

So, the sequence  $(y_n)$  is bounded above by 1. Further,

$$\begin{aligned} y_{n+1} - y_n &= \frac{1}{2n+1} + \frac{1}{2n+2} - \frac{1}{n+1} \\ &= \frac{1}{2n+1} - \frac{1}{2(n+1)} \\ &= \frac{1}{2(n+1)(2n+1)} \\ y_{n+1} - y_n &\geq 0. \end{aligned}$$

From the above inequality, we see that  $(y_n)$  is an increasing sequence. Therefore, by Monotone Convergence Theorem, it converges.

7. (**Abbott 2.4.2**) Consider the sequence defined by  $y_1 = 1$  and  $y_{n+1} = 3 - \frac{1}{y_n}$ . Prove that  $(y_n)$  converges and find  $y = \lim y_n$ .

**Proof.** Computing few terms of  $(y_n)$  suggests us that it is an increasing sequence bounded above by 3.

Suppose  $y_n \geq y_{n-1}$  for some  $n$  then  $y_{n+1} = 3 - \frac{1}{y_n} \geq 3 - \frac{1}{y_{n-1}} = y_n$ . Thus,  $y_{n+1} \geq y_n$  for all  $n \in \mathbb{N}$ .

Suppose  $y_n \leq 3$ , and  $(y_n)$  is an increasing sequence with  $y_1 = 1$  so  $1/y_n \geq 1/3$  then  $y_{n+1} = 3 - \frac{1}{y_n} \leq 3 - \frac{1}{3} < 3$ .

Therefore, by Monotone Convergence Theorem it converges. Taking the limit the the side of  $y_{n+1} = 3 - \frac{1}{y_n}$  gives us,  $y^2 - 3y + 1 = 0$ , and its solutions are  $y = 2.618033\dots$  and  $y = 0.381966\dots$ . Rejecting  $y = 0.381966\dots$  gives us  $y = \lim y_n = 2.618033\dots$ .